steel/Zeta.Steel.SafeMain.fsti
@@ -4,34 +4,30 @@ module M = Zeta.Steel.Main
 open Steel.ST.Util
 
 val handle_pts_to
-  (p: perm)
   (ts: M.top_level_state)
 : Tot vprop
 
 val gather
   (#opened: _)
-  (p1: perm)
   (ts1: M.top_level_state)
-  (p2: perm)
   (ts2: M.top_level_state)
 : STGhost unit opened
-    (handle_pts_to p1 ts1 `star` handle_pts_to p2 ts2)
-    (fun _ -> handle_pts_to (p1 `sum_perm` p2) ts1)
+    (handle_pts_to ts1 `star` handle_pts_to ts2)
+    (fun _ -> handle_pts_to ts1)
     True
     (fun _ -> ts1 == ts2)
 
 val share
   (#opened: _)
-  (p: perm)
   (ts: M.top_level_state)
 : STGhostT unit opened
-    (handle_pts_to p ts)
-    (fun _ -> handle_pts_to (half_perm p) ts `star` handle_pts_to (half_perm p) ts)
+    (handle_pts_to ts)
+    (fun _ -> handle_pts_to ts `star` handle_pts_to ts)
 
 [@@__reduce__]
 let init_post_true : vprop =
   exists_ (fun ts ->
-    handle_pts_to full_perm ts `star`
+    handle_pts_to ts `star`
     M.core_inv ts `star`
     M.all_logs ts (Map.const (Some Seq.empty))
   )
@@ -53,7 +49,7 @@ module V = Zeta.Steel.Verifier
 module A = Steel.ST.Array
 module AT = Zeta.Steel.ApplicationTypes
 
-val verify_log (#p: perm)
+val verify_log
                (#t:Ghost.erased M.top_level_state)
                (tid:_)
                (#entries:Ghost.erased AEH.log)
@@ -65,20 +61,20 @@ val verify_log (#p: perm)
                (#out_bytes:Ghost.erased AT.bytes)
                (output:U.larray U8.t out_len)
   : STT (option (v:V.verify_result { V.verify_result_complete len v }))
-    (handle_pts_to p t `star`
+    (handle_pts_to t `star`
      M.core_inv t `star`
      A.pts_to input log_perm log_bytes `star`
      A.pts_to output full_perm out_bytes `star`
      M.log_of_tid t tid entries)
     (fun res ->
-       handle_pts_to p t `star`
+       handle_pts_to t `star`
        M.verify_post t tid entries log_perm log_bytes len input out_len out_bytes output res)
 
-val max_certified_epoch (#p: perm)
+val max_certified_epoch
                         (#t:Ghost.erased M.top_level_state)
                         (_: unit)
   : STT AEH.max_certified_epoch_result
-        (handle_pts_to p t)
+        (handle_pts_to t)
         (fun res ->
-           handle_pts_to p t `star`
+           handle_pts_to t `star`
            M.read_max_post t res)
